Add a soundness result under usemantics

isabelle/Model.thy
@@ -17,6 +17,7 @@ definition is_env :: \<open>'a set \<Rightarrow> (nat \<Rightarrow> 'a) \<Righta
   \<open>is_env u e \<equiv> \<forall>n. e n \<in> u\<close>
 
 text \<open>A formula only needs to be valid for the "real" environments\<close>
+(* TODO: change this *)
 definition uvalid :: \<open>'a set \<Rightarrow> fm \<Rightarrow> bool\<close> where
   \<open>uvalid u p \<equiv> \<forall>e f g. is_env u e \<longrightarrow> usemantics u e f g p\<close>
 
@@ -37,8 +38,69 @@ lemma uvalid_semantics:
   using assms is_env_UNIV usemantics_UNIV unfolding uvalid_def
   by blast
 
+lemma uupd_lemma [iff]: \<open>n \<notin> params p \<Longrightarrow> usemantics u e (f(n := z)) g p \<longleftrightarrow> usemantics u e f g p\<close>
+  by (induct p arbitrary: e) simp_all
+
+text \<open>The semantics of substituting variable i by term t in formula a are well-defined\<close>
+lemma usubst_lemma [iff]:
+  \<open>usemantics u e f g (subst a t i) \<longleftrightarrow> usemantics u (SeCaV.shift e i (semantics_term e f t)) f g a\<close>
+  by (induct a arbitrary: e i t) simp_all
+
+subsection \<open>Soundness of SeCaV\<close>
+
+definition is_fdenot :: \<open>'a set \<Rightarrow> (nat \<Rightarrow> 'a list \<Rightarrow> 'a) \<Rightarrow> bool\<close> where
+  \<open>is_fdenot u f \<equiv> \<forall>i l. list_all (\<lambda>x. x \<in> u) l \<longrightarrow> f i l \<in> u\<close>
+
+lemma usemantics_term [simp]:
+  assumes \<open>is_env u e\<close> \<open>is_fdenot u f\<close>
+  shows \<open>semantics_term e f t \<in> u\<close> \<open>list_all (\<lambda>x. x \<in> u) (semantics_list e f l)\<close>
+  using assms by (induct t and l rule: semantics_term.induct semantics_list.induct)
+    (simp_all add: is_env_def is_fdenot_def)
+
+lemma is_env_shift [simp]: \<open>is_env u e \<Longrightarrow> x \<in> u \<Longrightarrow> is_env u (SeCaV.shift e v x)\<close>
+  unfolding is_env_def SeCaV.shift_def by simp                  
+
+lemma is_fdenot_shift [simp]: \<open>is_fdenot u f \<Longrightarrow> x \<in> u \<Longrightarrow> is_fdenot u (f(i := \<lambda>_. x))\<close>
+  unfolding is_fdenot_def SeCaV.shift_def by simp
+
+theorem sound_usemantics:
+  assumes \<open>\<tturnstile> z\<close> \<open>is_env u e\<close> \<open>is_fdenot u f\<close>
+  shows \<open>\<exists>p \<in> set z. usemantics u e f g p\<close>
+  using assms
+proof (induct arbitrary: f rule: sequent_calculus.induct)
+  case (10 i p z)
+  then show ?case
+  proof (cases \<open>\<forall>x \<in> u. usemantics u e (f(i := \<lambda>_. x)) g (sub 0 (Fun i []) p)\<close>)
+    case False
+    moreover have \<open>\<forall>x \<in> u. \<exists>p \<in> set (sub 0 (Fun i []) p # z). usemantics u e (f(i := \<lambda>_. x)) g p\<close>
+      using 10 is_fdenot_shift by metis
+    ultimately have \<open>\<exists>x \<in> u. \<exists>p \<in> set z. usemantics u e (f(i := \<lambda>_. x)) g p\<close>
+      by fastforce
+    moreover have \<open>list_all (\<lambda>p. i \<notin> params p) z\<close>
+      using 10 by simp
+    ultimately show ?thesis
+      using 10 Ball_set insert_iff list.set(2) uupd_lemma by metis
+  qed simp
+next
+  case (11 i p z)
+  then show ?case
+  proof (cases \<open>\<forall>x \<in> u. usemantics u e (f(i := \<lambda>_. x)) g (Neg (sub 0 (Fun i []) p))\<close>)
+    case False
+    moreover have
+      \<open>\<forall>x \<in> u. \<exists>p \<in> set (Neg (sub 0 (Fun i []) p) # z). usemantics u e (f(i := \<lambda>_. x)) g p\<close>
+      using 11 is_fdenot_shift by metis
+    ultimately have \<open>\<exists>x \<in> u. \<exists>p \<in> set z. usemantics u e (f(i := \<lambda>_. x)) g p\<close>
+      by fastforce
+    moreover have \<open>list_all (\<lambda>p. i \<notin> params p) z\<close>
+      using 11 by simp
+    ultimately show ?thesis
+      using 11 Ball_set insert_iff list.set(2) uupd_lemma by metis
+  qed simp
+qed fastforce+
+
 section \<open>Machinery\<close>
 
+(* TODO: remove these? *)
 text \<open>A term is closed wrt. scope m if it contains no variables that have de Bruijn indices at or above m\<close>
 primrec closedt where
   \<open>closedt m (Var n) = (n < m)\<close>
@@ -63,11 +125,6 @@ lemma closedt_usemantics_id [simp]:
   \<open>semantics_list e Fun ts = ts\<close>
   using assms by (induct t and ts rule: semantics_term.induct semantics_list.induct)
     (simp_all add: assms)
-
-text \<open>The semantics of substituting variable i by term t in formula a are well-defined\<close>
-lemma usubst_lemma [iff]:
-  \<open>usemantics u e f g (subst a t i) \<longleftrightarrow> usemantics u (SeCaV.shift e i (semantics_term e f t)) f g a\<close>
-  by (induct a arbitrary: e i t) simp_all
 
 text \<open>If t is a term in some argument list ts, t is also in the list of subterms of a function
 applied to those arguments\<close>
@@ -282,6 +339,12 @@ proof
       using assms by (metis someI equals0I)
   qed
 qed
+
+(* TODO: this does not hold *)
+lemma
+  assumes \<open>terms S \<noteq> {}\<close>
+  shows \<open>is_fdenot (terms S) Fun\<close>
+  unfolding is_fdenot_def list_all_def sorry
 
 text \<open>If S is a Hintikka set containing only closed formulas, then we can construct a countermodel
 for any closed formula using our alternate semantics and a Herbrand interpretation\<close>
